---
layout: post
title: "Fixed Point Iteration"
use_math: true
lang: en
tags: notes, convex-optimization
desc: This note summarize the Section 5.1-5.2 of Bauschke and Combettes (2011). The key result is the weak convergence of Krasnosel'skii–Mann (KM) Iteration, which is an fixed point algorithm of non-expansive operator mapping from a convex and closed set into itself. This result relies on that (1) weak convergence implies fixed point and (2) Fejér Monotonicity implies weak convergence.
---

<br>

Reference

Bauschke, H. H., & Combettes, P. L. (2011). *Convex analysis and monotone operator theory in Hilbert spaces* (Vol. 408). New York: Springer. 

<br>

This note summarize the [Section 5.1-5.2](https://link.springer.com/chapter/10.1007/978-1-4419-9467-7_5) of [Bauschke and Combettes (2011)](https://link.springer.com/book/10.1007/978-1-4419-9467-7). The key result is the weak convergence of Krasnosel'skii–Mann (KM) Iteration, which is an fixed point algorithm of non-expansive operator mapping from a convex and closed set into itself. This result relies on that (1) weak convergence implies fixed point (see Proposition 4.18) and (2) Fejér Monotonicity implies weak convergence (see Proposition 5.5). As a generalization, the non-expansiveness can be replaced by $\alpha$-averaging. 

<br>

## 1. Fejér Monotone Sequence

**Def. 5.1 (Fejér Monotonicity)** Let $C$ be a nonemoty subset of $\mathcal{H}$ and let $(x_n)$ be a sequence in $\mathcal{H}$. Then $(x_n)$ is Fejér monotone w.r.t. $C$ if 


$$
\|x_{n+1}-x\| \le \|x_n-x\|
$$


for all $x\in C$ and $n\in N$. 

**Example 5.2** A bounded increasing sequence $(x_n)$ is Fejér Monotone with respect to the set $(\sup x_n, +\infty)$. 

**Definition (Quasi-nonexpansiveness)** For any $\emptyset\not=D\subset\mathcal{H}$, an operator $T:D\to D$ such that $\text{Fix}(T)\not=\emptyset$ is [quasi-nonexpansive](https://www.cambridge.org/core/services/aop-cambridge-core/content/view/S144678870001123X) if  


$$
\|Tx-p\| \le \|x-p\|
$$


for all $x\in D$ and $p\in\text{Fix}(T)$. 

**Note.** Non-expansiveness implies quasi-non-expansiveness: 

$$
\|Tx - Tp\| \le \|x-p\|
\Rightarrow
\|Tx - p\| \le \|x - p\|
$$

for all $p\in\text{Fix}(T)$. 

**Example 5.3** Let $\emptyset\not=D\subset\mathcal{H}$ and let $T:D\to D$ be a quasi-nonexpansive operator such that $\text{Fix}(D)\not=\emptyset$. Then $(x_n)$ generated by the fixed point iterations of $T$ is Fejér Monotone. 

**Proposition 5.4 (Fejér monotonicity; General Set)** Let $\emptyset\not=C\subset\mathcal{H}$. Suppose $(x_n)\subset\mathcal{H}$ is Fejér monotone with respect to $C$. Then 

i) $(x_n)$ is bounded by $B(x,\Vert x_0-x\Vert)$ for any $x\in C$ 

***Proof.*** By definition 5.1. 

ii) For every $x\in C$ we have $(\Vert x_n-x \Vert)$ converges 

***Proof.*** By definition 5.1. 

iii) $(d_C(x_n))$ is decreasing and converges. 

***Proof.*** By contradiction. If $d_C(x_{n+1}) > d_C(x_n)$ for some $n\in N$, then 

$$
\|x_{n+1}-P_C(x_n)\| \ge \|x_{n+1}-P_C(x_{n+1})\| > \|x_n-P_C(x_n)\|
$$

iv) $\Vert x_{n+m}-x_n \Vert \le 2d_C(x_n)$ for all $m,n\in N$. 

***Proof.*** $\Vert x_{n+m}-x_n \Vert \le \Vert x_{n+m}-x \Vert + \Vert x_n-x \Vert \le 2\Vert x_n-x \Vert$ for all $x\in C$. 

<br>

## 2. Shadow of Fejér Monotone Sequence

**Proposition 5.7 (Shadow Sequence; Fejér monotonicity; Closed Convex Set)** Let $\emptyset\not=C\subset\mathcal{H}$ is convex and closed. Suppose $(x_n)\subset\mathcal{H}$ is Fejér monotone with respect to $C$. Then the shadow sequence $(P_C(x_n))$ converges strongly to a point $z\in C$. 

***Proof.*** For any $m, n\in N$ we have 

$$
\begin{aligned}
&\|P_C(x_m)-P_C(x_{n+m})\|^2\\
= &\|P_C(x_n)-x_{n+m}\|^2 + \|x_{n+m}-P_C(x_{n+m})\|^2 + 2\langle P_C(x_n)-x_{n+m}, x_{n+m}-P_C(x_{n+m}) \rangle\\
\le &\|P_C(x_n)-x_n\|^2 + d_C(x_{n+m})^2\\
&+ 2\langle P_C(x_n)-P_C(x_{n+m}), x_{n+m}-P_C(x_{n+m}) \rangle\\
&+ 2\langle P_C(x_{n+m})-x_{n+m}, x_{n+m}-P_C(x_{n+m}) \rangle\\
\le &d_C(x_n)^2 - d_C(x_{n+m})^2
\end{aligned}
$$

The first inequality is because $\Vert P_C(x_n)-x_{n+m}\Vert \le \Vert P_C(x_n)-x_n\Vert$ (Fejér monotonicity). The second inequality is because $\langle P_C(x_n)-P_C(x_{n+m}), x_{n+m}-P_C(x_{n+m}) \rangle \le 0$ (metric projection). By 5.4 (iii) we have $(d_C(x_n))$ decreasing and converge, $(P_C(x_n))$ is a Cauchy sequence. 

**Proposition 5.9 (Shadow Sequence; Fejér monotonicity; Closed Affine Subspace)** Let $C\subset\mathcal{H}$ is a closed affine subspace. Suppose $(x_n)\subset\mathcal{H}$ is Fejér monotone with respect to $C$. Then $P_C(x_n) = P_C(x_0)$ for all $n\in N$. 

***Proof.*** For any $n\in N$ and $\alpha \in R$ define $y_\alpha = \alpha P_C(x_0) + (1-\alpha) P_C(x_n) \in C$. Then for all $\alpha \in R$ and $n\in N$ we have 

$$
\langle y_\alpha - P_C(x_n), x_n - P_C(x_n) \rangle \le 0 
\Rightarrow
\alpha \langle P_C(x_0) - P_C(x_n), x_n - P_C(x_n) \rangle \le 0
$$

which implies that $y_\alpha - P_C(x_n) \perp x_n - P_C(x_n)$. We have 

$$
\begin{aligned}
\alpha^2 \|P_C(x_n) - P_C(x_0)\|^2 
&= \|P_C(x_n) - y_\alpha\|^2\\
&\le \|x_n-P_C(x_n)\|^2 + \|P_C(x_n)- y_\alpha\|^2\\
&= \|x_n - y_\alpha\|^2\\
&\le \|x_0 - y_\alpha\|^2\\
&= \|x_0  - P_C(x_0)\|^2 + \|P_C(x_0) - y_\alpha\|^2\\
&= d_C(x_0)^2 + (1-\alpha)^2\|P_C(x_n)-P_C(x_0)\|^2
\end{aligned}
$$

which implies that $(2\alpha - 1) \Vert P_C(x_n) - P_C(x_0)\Vert^2 \le d_C(x_0)^2$. Letting $\alpha \to +\infty$ and we have $P_C(x_n) = P_C(x_0)$. 

<br>

## 3. Convergence of Fejér Monotone Sequence

**Proposition 5.10 (Convergence; Fejér monotonicity; Nonempty Interior; Raik)** Let $C\subset\mathcal{H}$ such that $\text{int}(C)\not=\emptyset$. Suppose $(x_n)\subset\mathcal{H}$ is Fejér monotone with respect to $C$. Then $(x_n)$ converges strongly and $\sum_n\Vert x_{n+1}-x_n \Vert < +\infty$. 

***Proof.*** Pick $x\in \text{int}(C)$ and $\rho > 0$ such that $B(x,\rho) \subset C$. Define a sequence $(z_n)\subset B(x,\rho)$ by 

$$
z_n = \begin{cases}
x, &x_{n+1} = x_n\\
x - \rho\frac{x_{n+1}-x_n}{\|x_{n+1}-x_n\|},&\text{otherwise}
\end{cases}
$$

Then $\Vert x_{n+1}-z_n \Vert^2 \le \Vert x_n-z_n \Vert^2$ for all $(x_n)$ that is Fejér monotone with respect to $C$ and for all $n\in N$. We have 

$$
\begin{aligned}
(\|x_{n+1}-x\| + \rho)^2 &\le (\|x_n-x\| - \rho)^2\\
\Rightarrow\quad
\|x_{n+1}-x\|^2 + 2\rho \|x_{n+1}-x\| &\le \|x_n - x\|^2 - 2\rho\|x_n - x\|\\
\Rightarrow\quad\quad\quad\quad\quad\quad\quad\quad
\|x_{n+1} - x\|^2 &\le \|x_n - x\|^2 - 2\rho (\|x_n - x\| + \|x_{n+1} - x\|)\\
\Rightarrow\quad\quad\quad\quad\quad\quad\quad\quad
\|x_{n+1} - x\|^2 &\le \|x_n - x\|^2 - 2\rho \|x_{n+1} - x_n\|
\end{aligned}
$$

Thus 

$$
\sum_{n\in N}\|x_{n+1}-x_n\| \le \left(\frac{1}{2\rho}+1\right)\cdot\|x_0-x\|^2
$$

and $(x_n)$ is therefore a Cauchy sequence. 

**Proposition 5.11 (Convergence; Fejér monotonicity; Closed Convex Set)** Let $\emptyset\not=C\subset\mathcal{H}$ is convex and closed. Suppose $(x_n)\subset\mathcal{H}$ is Fejér monotone with respect to $C$. Then the following are equivalent 

i) $(x_n)$ converges strongly to a point in $C$. 

ii) $(x_n)$ possesses a strong sequential cluster point in $C$. 

iii) $\underline{\lim}d_C(x_n) = 0$. 

***Proof.*** 

i) $\Rightarrow$ ii): Statement ii) is equivalent to say that $(x_n)$ has a sub-sequence that converges to a point in $C$. 

ii) $\Rightarrow$ iii): Suppose $x_{k_n}\to x\in C$ then $d_C(x_{k_n}) \le \Vert x_{k_n} - x \Vert \to 0$. 

iii) $\Rightarrow$ i): By 5.4 (iii) we know $(d_C(x_n))$ is decreasing and convergent, then $\underline{\lim} d_C(x_n) = 0$ implies that $d_C(x_n)\to 0$. By proposition 5.7 we have $(P_C(x_n))$ converges strongly to some point in $C$, say $P_C(x_n) \to x\in C$, then 

$$
\|x_n - x\| \le \|x_n - P_C(x_n)\| + \|P_C(x_n)-x\| \to 0
$$

**Proposition 5.12 (Linear Convergence; Fejér monotonicity; Closed Convex Set)** Let $\emptyset\not=C\subset\mathcal{H}$ is convex and closed. Suppose $(x_n)\subset\mathcal{H}$ is Fejér monotone with respect to $C$ and there exists some $\kappa\in[0,1)$ such that for all $n\in N$ we have 

$$
d_C(x_{n+1}) \le \kappa \cdot d_C(x_n)
\tag{5.7}
$$

Then $(x_n)$ converges linearly to a point $x\in C$; more precisely, for all $n\in N$ we have 

$$
\|x_n-x\| \le 2 \kappa^n d_C(x_0)
\tag{5.8}
$$

***Proof.*** Condition (5.7) implies $\underline{\lim}d_C(x_n) = 0$ which, by Proposition 5.11, implies that $(x_n)$ converges strongly to a point in $C$, say $x_n\to x\in C$. Proposition 5.4 (iv) says for all $m,n\in N$ we have 

$$
\|x_{n} - x_{n+m}\| \le 2d_C(x_n)
$$

Let $m\to +\infty$ and we have $\Vert x_n - x \Vert \le 2d_C(x_n) \le 2\kappa^1 d_C(x_{n-1}) \le ... \le 2 \kappa^n d_C(x_0)$. 

<br>

## 4. Weak Convergence 

**Definition (Weak Convergence in Hilbert Space)** A sequence $(x_n)\subset\mathcal{H}$ is said to converge weakly to a point $x\in \mathcal{H}$ if 

$$
\langle x_n, y \rangle \to \langle x, y \rangle,
\quad
\forall y\in \mathcal{H}.
$$

The notation $x_n \rightharpoonup x$ is sometimes used to denote this kind of convergence. Referred from [Wikipedia](https://en.wikipedia.org/wiki/Weak_convergence_(Hilbert_space)). 

**Corollary 4.18 (Fixed Point; Weak Convergence; Asymptotic regularity)** Let $\emptyset\not=D\subset\mathcal{H}$ that is closed and convex and let $T:D\to \mathcal{H}$ be a non-expansive operator. If there exists $(x_n)\subset D$ and $x\in \mathcal{H}$ such that $x_n\rightharpoonup x$ and $x_n-T(x_n)\to 0$, then $x\in\text{Fix}(T)$. 

**Theorem 5.5 (Weak Convergence; Fejér Monotonicity)** Let $\emptyset\not=C\subset\mathcal{H}$ and $(x_n)\subset\mathcal{H}$ is Fejér monotone with respect to $C$. Suppose every weak sequential cluster point of $(x_n)$ belongs to $C$. Then $x_n\rightharpoonup x$. 

**Proposition 5.13 (Weak Convergence; Asymptotic regularity; Non-expansiveness)** Let $\emptyset\not=D\subset\mathcal{H}$ that is closed and convex and let $T:D\to D$ be a non-expansive operator with $\text{Fix}(T)\not=\emptyset$. Let $x_0 \in D$. Set 

$$
x_{n+1} = T(x_n)
\tag{5.9}
$$

and suppose that $x_{n}-T(x_n) \to 0$. Then 

i) $(x_n)$ converges weakly to a point in $\text{Fix}(T)$. 

ii) Suppose that $D = -D$ and that $T$ is odd: $T(-x) = -T(x)$ for all $x\in D$. Then $(x_n)$ converges strongly to a point in $\text{Fix}(T)$. 

***Proof.*** By Example 5.3 we have $(x_n)$ is Fejér monotone with respect to $\text{Fix}(T)$. 

i) Let $x$ to be a weak cluster point such that $x_{k_n} \rightharpoonup x$. Since $x_{k_n}-T(x_{k_n})\to 0$ we have $x\in \text{Fix}(T)$ by Corollary 4.18. Then by Theorem 5.5 we have $x_n\rightharpoonup \tilde{x} \in \text{Fix}(T)$. 

ii) Since $D = -D$ and $D$ is convex we must have $0 = 0.5x + 0.5(-x)\in D$ for all $x\in D$. Since $T$ is odd we must have $T(0) = T(-0) = -T(0) \Rightarrow T(0) = 0$. Thus, $0\in\text{Fix}(T)$. Thus, by Fejér monotonicity we have $\Vert x_{n+1} \Vert \le \Vert x_n \Vert$. Thus, $(\Vert x_n \Vert)$ is decreasing and converges to some point $\ell \ge 0$. For any $m,n\in N$ we have 

$$
\|x_{n+m+1} + x_{n+1}\| = \|T(x_{n+m})-T(-x_n)\| \le \|x_{n+m}+x_n\|
\tag{5.10}
$$

Thus, $(\Vert x_{n+m}+x_n \Vert)_{n\in N}$ is decreasing for all given $m\in N$. Also we have the identity 

$$
\|x_{n+m}+x_n\|^2 = 2(\|x_{n+m}\|^2+\|x_m\|^2) - \|x_{n+m}-x_n\|^2
\tag{5.11}
$$

Since $T(x_n)-x_n\to 0$ we have $\lim_{n}\Vert x_{n+m}-x_n \Vert=0$. Thus, $\Vert x_{n+m}+x_n \Vert^2 \downarrow 2(\ell^2+\Vert x_m \Vert^2)$ as $n\to+\infty$ for any given $m\in N$. Thus, $\Vert x_{n+m}-x_n \Vert^2\to 4\ell^2-4\ell^2 = 0$ as $m,n\to+\infty$. Thus, $(x_n)$ is a Cauchy sequence and $x_n\to x\in\mathcal{H}$. Since $x\leftarrow x_{n+1}=T(x_n)\to T(x)$ we have $x\in\text{Fix}(T)$. 

<br>

## 5. Krasnosel'skii–Mann (KM) Iteration

**Corollary (Identity)** For any $x, y\in\mathcal{H}$ and $\alpha\in R$ it is easy to verify that 

$$
\|\alpha x + (1-\alpha)y\|^2 + \alpha(1-\alpha)\|x-y\|^2 = \alpha\|x\|^2 + (1-\alpha)\|y\|^2
$$

**Proposition 5.14 (Weak Convergence; KM Algorithm)** Let $\emptyset\not=D\subset\mathcal{H}$ is convex and closed and let $T:D\to D$ be a non-expansive operator with $\text{Fix}(T)\not=\emptyset$. Let $(\lambda_n)\subset[0,1]$ with $\sum_n\lambda_n(1-\lambda_n) = +\infty$. Let $x_0\in D$. Set 

$$
x_{n+1} = x_n + \lambda_n(T(x_n) - x_n)
\tag{5.12}
$$

Then the following holds: 

i) $(x_n)$ is Fejér monotone w.r.t. $\text{Fix}(T)$. 

ii) $(Tx_n - x_n)$ converges strongly to zero. 

iii) $(x_n)$ converges weakly to a point in $\text{Fix}(T)$. 

***Proof.*** Since $x_0\in D$ and $D$ is convex, (5.12) generates a well-defined sequence in $D$. 

i) For any $y\in \text{Fix}(T)$ and $n\in N$ we have 

$$
\begin{aligned}
\|x_{n+1}-y\|^2 
&= \|(1-\lambda_n)(x_n-y) + \lambda_n(Tx_n-y)\|^2\\
&= (1-\lambda_n)\|x_n-y\|^2+\lambda_n\|Tx_n-Ty_n\|^2 - \lambda_n(1-\lambda_n)\|Tx_n-x_n\|^2\\
&\le \|x_n-y\|^2 - \lambda_n(1-\lambda_n)\|Tx_n-x_n\|^2
\end{aligned}
\tag{5.13}
$$

The inequality is by the non-expansiveness of $T$. 

ii) From (5.13) we have $\lambda_n(1-\lambda_n)\Vert Tx_n-x_n \Vert^2 \le \Vert x_n-y \Vert^2 - \Vert x_{n+1}-y \Vert^2$. Then 

$$
\sum_n \lambda_n(1-\lambda_n)\|Tx_n-x_n\|^2 \le \|x_0-y\|^2 
$$

Since $\sum_n\lambda_n(1-\lambda_n) = +\infty$ we must have $\underline{\lim}\Vert Tx_n-x_n \Vert=0$. And 

$$
\begin{aligned}
\|Tx_{n+1}-x_{n+1}\|
&= \|Tx_{n+1}-Tx_n+(1-\lambda_n)(Tx_n-x_n)\|\\
&\le \|x_{n+1}-x_n\| + (1-\lambda_n)\|Tx_n-x_n\|\\
&= \|Tx_n-x_n\|
\end{aligned}
\tag{5.14}
$$

Consequently $(Tx_n-x_n)\downarrow 0$. 

iii) For any $x\in D$ such that $x_{k_n}\rightharpoonup x$ we have $x\in \text{Fix}(T)$ by Corollary 4.18. Moreover $(x_n)$ is Fejér monotone w.r.t. $\text{Fix}(T)$. Thus, by Proposition 5.5 we have $x_n\rightharpoonup x$. 

<br>

## 6. $\alpha$-Averaged Operator

**Definition 4.23 ($\alpha$-Averaged Operator)** Let $\emptyset\not=D\subset\mathcal{H}$ and let $T:D\to\mathcal{H}$. Let $\alpha\in(0,1)$. Then $T$ is called $\alpha$-averaged if there exists a non-expansive operator $R:D\to\mathcal{H}$ such that $T = (1-\alpha)\text{Id}+\alpha R$. 

**Proposition 4.24 (Properties of $\alpha$-Averaged Operator - 1)** Let $\emptyset\not=D\subset\mathcal{H}$ and $T:D\to\mathcal{H}$. Let $\alpha\in(0,1)$. Then 

i) If $T$ is $\alpha$-averaged then it is non-expansive. 

ii) If $T$ is non-expansive it is NOT necessarily averaged. 

iii) $T$ is firmly non-expansive iff it is $1/2$-averaged. 

**Proposition 4.25 (Properties of $\alpha$-Averaged Operator - 2)** Let $\emptyset\not=D\subset\mathcal{H}$ and $T:D\to\mathcal{H}$. Let $\alpha\in(0,1)$. Then the following are equivalent 

i) $T$ is $\alpha$-averaged. 

ii) $R\equiv(1-1/\alpha)\text{Id}+(1/\alpha)T$ is non-expansive. 

iii) $\Vert T(x)-T(y) \Vert^2 \le \Vert x-y \Vert^2 - \frac{1-\alpha}{\alpha} \Vert(\text{Id}-T)x-(\text{Id}-T)y \Vert^2$ for all $x, y\in D$. 

iv) $\Vert T(x) - T(y)\Vert^2 + (1-2\alpha)\Vert x-y\Vert^2 \le 2(1-\alpha)\langle x-y,T(x) - T(y)\rangle$ for all $x,y\in D$. 

**Proposition 5.15 (Weak Convergence; $\alpha$-Averaged Operator)** Let $\alpha\in[0,1]$ and $T:\mathcal{H}\to\mathcal{H}$ be an $\alpha$-averaged operator such that $\text{Fix}(T)\not=\emptyset$. Let $(\lambda_n)$ be a sequence in $[0,1/\alpha]$ with $\sum_n\lambda_n(1-\alpha\lambda_n)= +\infty$. Let $x_0\in\mathcal{H}$ and set 

$$
x_{n+1} = x_n + \lambda_n[T(x_n)-x_n]
\tag{5.15}
$$

Then the following hold: 

i) $(x_n)$ is Fejér monotone w.r.t. $\text{Fix}(T)$. 

ii) $(Tx_n - x_n)$ converges strongly to zero. 

iii) $(x_n)$ converges weakly to a point in $\text{Fix}(T)$. 

***Proof.*** 

Set $R = (1-1/\alpha)\text{Id}+1/\alpha T$ for all $n\in N$. Then $\text{Fix}(R) = \text{Fix}(T)$ by definition and $R$ is non-expansive by Proposition 4.25. Then (5.15) is 

$$
x_{n+1} = x_n +\alpha\lambda_n(Rx_n - x_n)
$$

Since $\alpha\lambda_n\in[0,1]$ and $\sum_n\alpha\lambda_n(1-\alpha\lambda_n) = +\infty$, the result follows Proposition 5.14. 

**Corollary 5.16 (Special Case: $1/2$-averaged)** Let $T:\mathcal{H}\to\mathcal{H}$ be a firmly non-expansive operator with $\text{Fix}(T)\not=\emptyset$. Let $(\lambda_n)$ be a sequence in $[0,2]$ with $\sum_n\lambda_n(2-\lambda_n) = +\infty$ and let $x_0\in\mathcal{H}$. Set $x_{n+1} = x_n +\lambda_n(Tx_n-x_n)$. Then 

i) $(x_n)$ is Fejér monotone w.r.t. $\text{Fix}(T)$. 

ii) $(Tx_n - x_n)$ converges strongly to zero. 

iii) $(x_n)$ converges weakly to a point in $\text{Fix}(T)$. 

***Proof.*** When $\alpha = 1/2$ and apply Proposition 4.24 (iii) and Proposition 5.15. 

**Example 5.17 (Special Case: $1/2$-averaged when $\lambda_n=1$)** Let $T:\mathcal{H}\to\mathcal{H}$ be a firmly non-expansive operator such that $\text{Fix}(T)\not=\emptyset$. Let $x_0\in\mathcal{H}$. Set $x_{n+1}=T(x_n)$. Then $(x_n)$ converges weakly to a point in $\text{Fix}(T)$. 

<br>



